proof: verify that there are no panics in read methods

coq_translation/default/examples/ink_contracts/Proofs/erc20.v
@@ -87,3 +87,107 @@ Proof.
   }
   { run_symbolic. }
 Qed.
+
+Module ReadMessage.
+  (** A message that only read the store. *)
+  Inductive t : Set -> Set :=
+  | total_supply : t ltac:(erc20.Balance)
+  | balance_of (owner : erc20.AccountId.t) : t ltac:(erc20.Balance)
+  | allowance (owner : erc20.AccountId.t) (spender : erc20.AccountId.t) :
+    t ltac:(erc20.Balance)
+  .
+
+  Definition dispatch {A : Set} (message : t A) : M (M.Val A) :=
+    let self : M.Val (ref erc20.Erc20.t) := Ref.Imm (Ref.mut_ref tt) in
+    match message with
+    | total_supply => erc20.Impl_erc20_Erc20_t_2.total_supply self
+    | balance_of owner =>
+      erc20.Impl_erc20_Erc20_t_2.balance_of self (Ref.Imm owner)
+    | allowance owner spender =>
+      erc20.Impl_erc20_Erc20_t_2.allowance
+        self
+        (Ref.Imm owner)
+        (Ref.Imm spender)
+    end.
+End ReadMessage.
+
+Module WriteMessage.
+  (** A message that can mutate the store. *)
+  Inductive t : Set :=
+  | transfer : erc20.AccountId.t -> ltac:(erc20.Balance) -> t
+  | approve : erc20.AccountId.t -> ltac:(erc20.Balance) -> t
+  | transfer_from :
+    erc20.AccountId.t ->
+    erc20.AccountId.t ->
+    ltac:(erc20.Balance) ->
+    t
+  .
+
+  Definition dispatch (message : t) : M (M.Val ltac:(erc20.Result unit)) :=
+    let self : M.Val (ref erc20.Erc20.t) := Ref.Imm (Ref.mut_ref tt) in
+    match message with
+    | transfer to value =>
+      erc20.Impl_erc20_Erc20_t_2.transfer
+        self
+        (Ref.Imm to)
+        (Ref.Imm value)
+    | approve spender value =>
+      erc20.Impl_erc20_Erc20_t_2.approve
+        self
+        (Ref.Imm spender)
+        (Ref.Imm value)
+    | transfer_from from to value =>
+      erc20.Impl_erc20_Erc20_t_2.transfer_from
+        self
+        (Ref.Imm from)
+        (Ref.Imm to)
+        (Ref.Imm value)
+    end.
+End WriteMessage.
+
+(** There are no panics with read messages. *)
+Lemma run_read_message_no_panic
+  (message : ReadMessage.t ltac:(erc20.Balance))
+  (storage : erc20.Erc20.t)
+  fuel :
+  let state := Some storage in
+  exists result,
+  Run.t
+    (ReadMessage.dispatch message fuel)
+    state
+    (* no errors in the result *)
+    (inl result)
+    (* the state does not change *)
+    state.
+Proof.
+  destruct message.
+  { eexists.
+    unfold ReadMessage.dispatch.
+    run_symbolic.
+  }
+  { destruct (Lib.Mapping.get owner storage.(erc20.Erc20.balances)) eqn:H_get; (
+      eexists;
+      unfold ReadMessage.dispatch;
+      run_symbolic; [
+        simpl;
+        rewrite H_get;
+        run_symbolic
+      | run_symbolic
+      | run_symbolic
+      ]
+    ).
+  }
+  { destruct (Lib.Mapping.get (owner, spender) storage.(erc20.Erc20.allowances))
+      eqn:H_get; (
+      eexists;
+      unfold ReadMessage.dispatch;
+      run_symbolic; [
+        simpl;
+        rewrite H_get;
+        run_symbolic
+      | run_symbolic
+      | run_symbolic
+      ]
+    ).
+  }
+Qed.
